Flapjack/Stack.lean
@@ -200,12 +200,12 @@ def wordToStackCallNoHandler (_perf : Bool) (target : Nat)
 def wordToStackCallWithHandlerInSection (perf : Bool) (target : Nat)
     (argumentCount frameOffset scratch : Nat)
     (returnCode handlerCode : StackProg α)
-    (returnLabel entryLabel sectionId handlerLabel exceptionLabel : Nat) : StackProg α :=
+    (returnLabel entryLabel handlerLabel handlerEntryLabel exceptionLabel : Nat) : StackProg α :=
   let callCode :=
     .call (some (returnCode, 0, returnLabel, entryLabel)) (.label target)
       (some (handlerCode, exceptionLabel, handlerLabel))
   stackSeq [
-    stackPushHandler perf sectionId handlerLabel scratch,
+    stackPushHandler perf handlerLabel handlerEntryLabel scratch,
     stackHandlerArgs perf (argumentCount + 1) frameOffset scratch,
     callCode
   ]
